src/ops/get.v
@@ -9,8 +9,8 @@ Require Import props.bineqs props.getbit spec.
 Definition get {n}(bs: BITS n)(k: 'I_n): bool
   := (andB (shrBn bs k) #1) == #1.
 
-Lemma get_repr:
-  forall n (k: 'I_n.+1)(bs: BITS n.+1) E, repr bs E -> get bs k = (k \in E).
+Lemma get_repr: forall n (k: 'I_n.+1)(bs: BITS n.+1) E, repr bs E -> 
+      get bs k = (k \in E).
 Proof.
   move=> n k bs E HE.
   rewrite /get andB_mask1 getBit_shrBn addn0=> //.
